updates

Veritas.Verifier.EAC.fst
@@ -636,8 +636,59 @@ let lemma_non_eac_instore_evictbm (#p:pos)
     EvictBM? (to_vlog_entry (invalidating_log_entry itsl))
    })
   : hash_collision_gen = 
-  admit()
+  let st = last_valid_eac_state itsl in   
+  let ee = invalidating_log_entry itsl in
+  assert(eac_add ee st = EACFail);
+  match st with
+  | EACInStore m v -> (
+    match ee with
+    | Evict (EvictBM k k' t) v' ->     
+      assert(DVal? v && v' <> v || m <> MAdd);        
+      let tsle = time_seq_ext itsl in
+      let i = max_eac_prefix tsle in
+      let (e,tid) = index itsl i in
 
+      let itsli = its_prefix itsl i in  
+      (* verifier thread state of tid after itsli *)
+      let vsi = verifier_thread_state itsli tid in
+
+      let itsli' = its_prefix itsl (i + 1) in
+      let vsi' = verifier_thread_state itsli tid in    
+      lemma_verifier_thread_state_extend itsli';  
+      assert(vsi' == t_verify_step vsi e);    
+      
+      (* the thread store of tid contains k *)
+      assert(store_contains (thread_store vsi) k);
+
+      let lidx = last_add_idx itsli k in
+      let ltid = last_add_tid itsli k in
+      let li = project_seq itsli in
+
+      lemma_eac_state_instore_addm itsli k;
+      assert(addm_of_entry (index li lidx) = m);
+      assert(add_method_of (thread_store vsi) k = m);
+      assert(add_method_of (thread_store vsi) k = MAdd);
+
+      if ltid = tid then (
+        assert(m = MAdd);
+        assert(DVal? v && v' <> v);
+        lemma_eac_state_instore itsli k;
+        assert(stored_value (thread_store vsi) k = v);
+
+        lemma_ext_evict_val_is_stored_val itsl i;      
+        assert(v' = stored_value (thread_store vsi) k);
+
+        hash_collision_contra()
+      )
+      else (    
+        (* only the store of last add contains the key k *)
+        lemma_eac_state_instore2 itsli k tid;
+        assert(not (store_contains (thread_store vsi) k));
+
+        (* ... which is a contradiction *)
+        hash_collision_contra()
+      )
+ )
 
 let lemma_non_eac_time_seq_implies_hash_collision 
   (#n:pos) 
